**2.a**

Distance 1: $2$ nodes: (2,1), (1,2)
Distance 2: $3$ nodes: (2,2), (1,3), (3,1)
Distance 3: $4$ nodes: (1,4), (4,1), (2,3), (3,2)

Distance $i$ :  $i + 1$ nodes $\forall \, 1 \le i \le n -1$
Distance $n$ :  $n$ nodes

For $i \ne n$, we can partition the distance $i$ into x and y distance. Because both distances add up to $i$, we just need to find the number of values we can assign to x distance. Including $0$, there are $i+1$ values we can assign to x distance, and thus there will be $i+1$ nodes of distance $i$. If $i = n$, the maximum x or y distance we can have is $n - 1$, thus we can have $n - 1 + 1 = n$ possible nodes.

**2.b**

$B_j$ consists of nodes of distance $1, 2, ... 2^j$.

For $0 \le j \lt log\, n$

$$\begin{align}
Number\, of\, nodes &= \sum^{2^j}_{k=1}(k + 1) \\
                &= \frac{2^j(2^j + 1)}{2} + 2^j\\
                &= 2^{2j - 1} + 2^j + 2^{j-1} \\
\end{align}
$$

For $j = log\, n$
$$\begin{align}
Number\, of\, nodes &= 2^{2j - 3} + 2^{j-1} + 2^{j-2}  + n
\end{align}
$$

**2.c**

$$\begin{align}
|R_j| &= |B_j| - |B_{j-1}|\\
      &= 2^{2j - 1} + 2^j + 2^{j-1}  - (2^{2j - 3} + 2^{j-1} + 2^{j-2} )\\
        &\approx 2^{2j-1}\\
\end{align}
$$

**2.d**

For $v \in R_j$, the probability of $u = (1,1)$ being connected by a random link, $$Pr(u\leftrightarrow v) \ge \frac{2^{-\alpha j}}{4ln(6n)}$$

Given that there is only one link, the probability that the link connects to some $v \in R_j$:

$$Pr(u \leftrightarrow R_j) \ge \frac{2^{2j - 1}2^{-\alpha j}}{4ln(6n)} / \sum^{log\, n}_{k=0} \frac{2^{2k - 1}2^{-\alpha k}}{4ln(6n)}$$

For $\alpha = 2$:
$$
\begin{align}
Pr(u \leftrightarrow R_j)
&\ge \frac{2^{2j - 1}2^{-2j}}{4ln(6n)} / \sum^{log\, n}_{k=0} \frac{2^{2k - 1}2^{-2k}}{4ln(6n)}\\
&= \frac{2^{-1}}{4ln(6n)} / \sum^{log\, n}_{k=0} \frac{2^{- 1}}{4ln(6n)}\\
&= \frac1{log\,n}\\
\end{align}$$

This value is independent of $j$

**2.e**
If $\alpha \ne 2$, the probability of the link connecting to a node in $R_j$ will be dependent on the value of j.

For $\alpha = 3$:
$$
\begin{align}
Pr(u \leftrightarrow R_j)
&\ge \frac{2^{2j - 1}2^{-3j}}{4ln(6n)} / \sum^{log\, n}_{k=0} \frac{2^{2k - 1}2^{-3k}}{4ln(6n)}\\
&= \frac{2^{-j-1}}{4ln(6n)} / \sum^{log\, n}_{k=0} \frac{2^{-k-1}}{4ln(6n)}\\
\end{align}$$

For smaller values of $j$, the larger the numerator. Thus closer nodes will be favoured.

For $\alpha = 1$:
$$
\begin{align}
Pr(u \leftrightarrow R_j)
&\ge \frac{2^{2j - 1}2^{-j}}{4ln(6n)} / \sum^{log\, n}_{k=0} \frac{2^{2k - 1}2^{-k}}{4ln(6n)}\\
&= \frac{2^{j-1}}{4ln(6n)} / \sum^{log\, n}_{k=0} \frac{2^{k-1}}{4ln(6n)}\\
\end{align}$$

For smaller values of $j$, the smaller the numerator. Thus further nodes will be favoured.
