###Exercise 4

####Part 1

$$x_1 + x_2 = C\\
p_1 = \frac{\delta}{dx_1} a\log x_1 = \frac{a}{x_1}\\
p_2 = \frac{\delta}{dx_2} b\log x_2 = \frac{b}{x_2}\\
$$

If

$$\lambda = \frac{a}{x_1} = \frac{b}{x_2}\\
x_1 = \frac{a}{b}x_2\\
(1+\frac{a}{b})x_2 = C\\
x_2 = \frac{b}{a+b}C\\
x_1 = \frac{a}{a+b}C\\
\lambda = \frac{a+b}{C} $$

####Part 2

Optimal welfare is obtained when for each user $U'(x) = c$

For user 1
$$\frac{a}{x_1} = c\\
x_1  = \frac{a}{c}$$



For user 2
$$\frac{b}{x_2} = c\\
x_2  = \frac{b}{c}$$



####Part 3

As the number of users increases, 

For case 1:

$$P(n) = \frac{an + b}{C}$$

For case 2:

$$P(n) = c$$

For the second case, the price will likely remain unchanged as the marginal capacity cost will regulate the price of the to maximise the utility of each individuals regardless of how many individuals are present.

####Part 4

This cost can be recovered from the user by charging each user a fixed cost of $B/2$. This, however can cause the potential problem by driving the user out if the fixed price happens to exceed his utility function.

####Part 5

Demand for user 1:

Differentiate
$$a \log x_1 - (g + hx_1) \\
\frac{a}{x_1} - h = 0\\
x_1 = \frac{a}{h}\\$$

Demand for user 2:

Differentiate
$$b \log x_2 - (g + hx_2) \\
\frac{b}{x_2} - h = 0\\
x_2 = \frac{b}{h}\\$$

If we push user 1's net utility to 0:

$$a \log x_1 - (g + hx_1) = 0\\
a \log \frac{a}{h} = g + h \frac{a}{h}\\
g = a \log \frac{a}{h} - a \\
g = a (\log \frac{a}{h} - 1) \\$$

Given the above g,

User 2's net utility would be:

$$b \log x_2 - (g + hx_2) = \\
b \log \frac{b}{h} - (a (\log \frac{a}{h} - 1) + b) = \\
b \log \frac{b}{h} - a \log \frac{a}{h} + a - b = \\
b (\log {b} - \log {h}) - (a (\log a - log h)) + a - b = \\
b\log b - a \log a - b \log h + a \log h + a - b = \\
b\log b - a \log a + (a - b)(1 + \log h)
$$
Since $b > a$, this implies that $b\log b - a \log a > 0$ and $(a - b)(1 + \log h) < 0$

If we set h to be sufficiently low such that $(a - b)(1 + \log h) > b\log b - a \log a$,
this would result in User 2 still enjoying net utility while User 1 does not.

On the other hand, if we were to push user 2's net utility to 0,

User 1's net utility would be given by,

$$a \log a - b \log b + (b - a)(1 + \log h)$$

This would require us to set h to large value instead.

Since the former is more feasible, it is easier for us to find a h that would result in
$(a - b)(1 + \log h) > b\log b - a \log a$.

This would imply that we should charge our users a price of:

$g + hx$ where $g = a (\log \frac{a}{h} - 1)$

User two would still benefit while User 1 does not.
