
###Exercise 3

$$E[n,p] = \frac{\frac{p^n}{n!}}{}$$

Sub $tp = p$ into Equation 1

$$e^{-t\rho}\sum^n_{k=0} (t\rho)^k / k! = \int^\infty_{tp}\frac{x^ne^{-x}}{n!}dx$$

Sub $t\rho = \rho, tn = n$ into $1/E[n,\rho]$


$$\frac{1}{E[tn,t\rho]} = \frac{\sum^{tn}_{i=0}\frac{t\rho^i}{i!}}{\frac{(t\rho)^n}{(tn)!}} \\
=\frac{(tn)!}{(t\rho)^n}e^{t\rho}\int^\infty_{tp}\frac{x^{tn}e^{-x}}{(tn)!}dx
\\=\frac{(tn)!}{(t\rho)^n}\frac{1}{(tn)!}e^{t\rho}\int^\infty_{tp}x^{tn}e^{-x}dx
\\=\frac{e^{t\rho}}{(t\rho)^n}\int^\infty_{tp}x^{tn}e^{-x}dx$$

Reindex $t\rho$ to 0

$$\frac{1}{E[tn,t\rho]}=\frac{e^{t\rho}}{(t\rho)^n}\int^\infty_0x^{tn}e^{-x}dx$$

Integrating $x^{tn}e^{-x}$, we get

$$\frac{1}{E[tn,t\rho]}=\frac{e^{t\rho}}{(t\rho)^n}\Gamma(tn + 1)$$

Since an exponential function increases at a far greater rate than a polynomial function, $\frac{e^{t\rho}}{(t\rho)^n}$ is an increasing function.

Since the gamma function is an increasing function as well, this implies that $\frac{1}{E[tn,t\rho]}$ is an increasing function as well.

As such, $E[tn,t\rho]$ is a strictly decreasing function in $t$, which implies that $E[2n,2ρ] < E[n,ρ]$.

> Written with [StackEdit](https://stackedit.io/).